

## Homogeneous Functions and Euler theorem

Consider the expression  $f(x, y) = a_0x_n + a_1x_{n-1}y + a_2x_{n-2}y_2 + \dots + a_ny_n \dots (1)$

The degree of each term in the above expression is 'n'. Such an expression is called a homogeneous function of degree 'n', Equation (i) can be written as  $f(x, y) = x^n f\left(\frac{y}{x}\right)$ .

**Note:**

A function  $f(x, y)$  is said to be a homogeneous function in  $x$  and  $y$  of degree 'n' if

$$f(tx, ty) = t^n f(x, y)$$

For example,  $f(x, y) = \frac{x^3 + y^3}{x - y}$

$$f(tx, ty) = \frac{t^3x^3 + t^3y^3}{tx - ty}$$

$$= \frac{t^3(x^3 + y^3)}{t(x - y)}$$

$$= \frac{t^2(x^3 + y^3)}{x - y}$$

$$f(tx, ty) = t^2 f(x, y)$$

$\therefore f(x, y)$  is a homogeneous function in of degree '2'.

### Euler's theorem on homogeneous function:

If  $u$  is a homogeneous function in  $x$  and  $y$  of degree 'n' then  $x \frac{\partial u}{\partial x} + y \frac{\partial u}{\partial y} = nu$

**Proof:**

Given 'u' is a homogeneous function of degree 'n' in  $x$  and  $y$

$$\therefore u(x, y) = x^n f\left(\frac{y}{x}\right)$$

$$\frac{\partial u}{\partial x} = nx^{n-1}f\left(\frac{y}{x}\right) + x^n f'\left(\frac{y}{x}\right)\left(-\frac{y}{x^2}\right)$$

$$= nx^{n-1}f\left(\frac{y}{x}\right) - yx^{n-2}f'\left(\frac{y}{x}\right)$$

and  $\frac{\partial u}{\partial x} = x^n f'\left(\frac{y}{x}\right)\left(\frac{1}{x}\right)$

$$= x^{n-1}f'\left(\frac{y}{x}\right)$$

Hence  $x \frac{\partial u}{\partial x} + y \frac{\partial u}{\partial y} = nx^n f\left(\frac{y}{x}\right) - yx^{n-1}f'\left(\frac{y}{x}\right) + yx^{n-1}f'\left(\frac{y}{x}\right)$

$$= nx^n f\left(\frac{y}{x}\right) = nu$$

$$\therefore x \frac{\partial u}{\partial x} + y \frac{\partial u}{\partial y} = nu$$

**Note:**

(i) If 'u' is a homogeneous function of three variables x, y and z of degree 'n', then the Euler's theorem is  $x \frac{\partial u}{\partial x} + y \frac{\partial u}{\partial y} + z \frac{\partial u}{\partial z} = nu$

(ii) Euler's extension theorem is  $x^2 \frac{\partial^2 u}{\partial x^2} + 2xy \frac{\partial^2 u}{\partial x \partial y} + y^2 \frac{\partial^2 u}{\partial y^2} = n(n-1)u$

**Example:**

**Verify Euler's theorem for the function  $u = (x^{\frac{1}{2}} + y^{\frac{1}{2}})(x^n + y^n)$**

**Solution:**

$$\text{Given } u(x, y) = (x^{\frac{1}{2}} + y^{\frac{1}{2}})(x^n + y^n)$$

$$U(tx, ty) = (t^{\frac{1}{2}}x^{\frac{1}{2}} + t^{\frac{1}{2}}y^{\frac{1}{2}})(t^n x^n + t^n y^n)$$

$$= t^{\frac{1}{2}}(x^{\frac{1}{2}} + y^{\frac{1}{2}})t^n(x^n + y^n)$$

$$= t^{n+\frac{1}{2}}(x^{\frac{1}{2}} + y^{\frac{1}{2}})(x^n + y^n)$$

$$u(tx, ty) = t^{n+\frac{1}{2}}u(x, y)$$

$\therefore u(x, y)$  is a homogeneous function in of degree ' $n + \frac{1}{2}$ '.

$\therefore$  Euler's theorem is  $x \frac{\partial u}{\partial x} + y \frac{\partial u}{\partial y} = (n + \frac{1}{2})u$

Verification: Consider L.H.S =  $x \frac{\partial u}{\partial x} + y \frac{\partial u}{\partial y}$

$$\frac{\partial u}{\partial x} = \frac{1}{2}x^{-\frac{1}{2}}(x^n + y^n) + nx^{n-1}(x^{\frac{1}{2}} + y^{\frac{1}{2}})$$

$$x \frac{\partial u}{\partial x} = \frac{1}{2}x^{\frac{1}{2}}(x^n + y^n) + nx^n(x^{\frac{1}{2}} + y^{\frac{1}{2}}) \dots (1)$$

$$\frac{\partial u}{\partial y} = \frac{1}{2}y^{-\frac{1}{2}}(x^n + y^n) + ny^{n-1}(x^{\frac{1}{2}} + y^{\frac{1}{2}})$$

$$y \frac{\partial u}{\partial y} = \frac{1}{2}y^{\frac{1}{2}}(x^n + y^n) + ny^n(x^{\frac{1}{2}} + y^{\frac{1}{2}}) \dots (2)$$

$$(1) + (2) \Rightarrow \text{L.H.S} = x \frac{\partial u}{\partial x} + y \frac{\partial u}{\partial y}$$

$$= \frac{1}{2}x^{\frac{1}{2}}(x^n + y^n) + nx^n(x^{\frac{1}{2}} + y^{\frac{1}{2}}) + \frac{1}{2}y^{\frac{1}{2}}(x^n + y^n) + ny^n(x^{\frac{1}{2}} + y^{\frac{1}{2}})$$

$$= \frac{1}{2}(x^{\frac{1}{2}} + y^{\frac{1}{2}})(x^n + y^n) + n(x^{\frac{1}{2}} + y^{\frac{1}{2}})(x^n + y^n)$$

$$= (n + \frac{1}{2})(x^{\frac{1}{2}} + y^{\frac{1}{2}})(x^n + y^n)$$

$$= (n + \frac{1}{2})u = \text{R.H.S}$$

Hence Euler's theorem is verified.

**Example:**

Verify Euler's theorem for the function  $u = \sin^{-1}\left(\frac{x}{y}\right) + \tan^{-1}\left(\frac{y}{x}\right)$

**Solution:**

$$\text{Given } u(x, y) = \sin^{-1}\left(\frac{x}{y}\right) + \tan^{-1}\left(\frac{y}{x}\right)$$

$$\begin{aligned} u(tx, ty) &= \sin^{-1}\left(\frac{tx}{ty}\right) + \tan^{-1}\left(\frac{ty}{tx}\right) \\ &= t^0 \left[ \sin^{-1}\left(\frac{x}{y}\right) + \tan^{-1}\left(\frac{y}{x}\right) \right] \end{aligned}$$

$$u(tx, ty) = t^0 u(x, y)$$

$\therefore u(x, y)$  is a homogeneous function in of degree '0'

$\therefore$  Euler's theorem is  $x \frac{\partial u}{\partial x} + y \frac{\partial u}{\partial y} = 0 \cdot u = 0$

Verification: Consider L.H.S =  $x \frac{\partial u}{\partial x} + y \frac{\partial u}{\partial y}$

$$\begin{aligned} \frac{\partial u}{\partial x} &= \frac{1}{\sqrt{1-\frac{x^2}{y^2}}} \times \frac{1}{y} + \frac{1}{1+\frac{y^2}{x^2}} \times \left(-\frac{y}{x^2}\right) \\ &= \frac{1}{\sqrt{y^2+x^2}} - \frac{y}{x^2+y^2} \end{aligned}$$

$$x \frac{\partial u}{\partial x} = \frac{x}{\sqrt{y^2+x^2}} - \frac{xy}{x^2+y^2} \dots (1)$$

$$\begin{aligned} \frac{\partial u}{\partial y} &= \frac{1}{\sqrt{1-\frac{x^2}{y^2}}} \times \left(-\frac{x}{y^2}\right) + \frac{1}{1+\frac{y^2}{x^2}} \times \frac{1}{x} \\ &= -\frac{x}{y\sqrt{y^2+x^2}} + \frac{x}{x^2+y^2} \end{aligned}$$

$$y \frac{\partial u}{\partial y} = -\frac{x}{\sqrt{y^2+x^2}} + \frac{xy}{x^2+y^2} \dots (2)$$

$$\begin{aligned} (1) + (2) \Rightarrow \text{L.H.S} &= x \frac{\partial u}{\partial x} + y \frac{\partial u}{\partial y} \\ &= \frac{x}{\sqrt{y^2+x^2}} - \frac{xy}{x^2+y^2} - \frac{x}{\sqrt{y^2+x^2}} + \frac{xy}{x^2+y^2} \\ &= 0 = \text{R.H.S} \end{aligned}$$

Hence Euler's theorem is verified.

**Example:**

If  $u = \tan^{-1}\left(\frac{x^3+y^3}{x-y}\right)$  then prove that  $x \frac{\partial u}{\partial x} + y \frac{\partial u}{\partial y} = \sin 2u$

**Solution:**

$$\text{Given } u(x, y) = \tan^{-1} \left( \frac{x^3 + y^3}{x - y} \right)$$

$$\tan u = \frac{x^3 + y^3}{x - y}$$

$$\text{Let } z = \tan u = \frac{x^3 + y^3}{x - y}$$

$$\text{Consider } z(x, y) = \frac{x^3 + y^3}{x - y}$$

$$z(tx, ty) = \frac{t^3 x^3 + t^3 y^3}{tx - ty} = t^2 z(x, y)$$

$\therefore z(x, y)$  is a homogeneous function in of degree '2'.

$$\therefore \text{ By Euler's theorem } x \frac{\partial z}{\partial x} + y \frac{\partial z}{\partial y} = 2 \cdot z$$

$$\text{Put } z = \tan u$$

$$x \frac{\partial(\tan u)}{\partial x} + y \frac{\partial(\tan u)}{\partial y} = 2 \tan u$$

$$x \sec^2 u \frac{\partial u}{\partial x} + y \sec^2 u \frac{\partial u}{\partial y} = 2 \tan u$$

$$x \frac{\partial u}{\partial x} + y \frac{\partial u}{\partial y} = 2 \frac{\sin u}{\cos u \sec^2 u}$$

$$= 2 \frac{\sin u}{\cos u} \cdot \frac{1}{\cos^2 u}$$

$$= 2 \sin u \cos u$$

$$= \sin 2u$$

Hence proved.

**Example:**

$$\text{If } u = \sin^{-1} \left( \frac{x+y}{\sqrt{x}+\sqrt{y}} \right), \text{ then prove that } x^2 \frac{\partial^2 u}{\partial x^2} + 2xy \frac{\partial^2 u}{\partial x \partial y} + y^2 \frac{\partial^2 u}{\partial y^2} = \frac{-\sin u \cos 2u}{4 \cos^3 u}$$

**Solution:**

$$\text{Given } u(x, y) = \sin^{-1} \left( \frac{x+y}{\sqrt{x}+\sqrt{y}} \right)$$

$$\sin u = \frac{x+y}{\sqrt{x}+\sqrt{y}}$$

$$\text{Let } z = \sin u = \frac{x+y}{\sqrt{x}+\sqrt{y}}$$

$$\text{Consider } z(x, y) = \frac{tx+ty}{\sqrt{t}\sqrt{x}+\sqrt{t}\sqrt{y}}$$

$$z(tx, ty) = t^{\frac{1}{2}} \left( \frac{x+y}{\sqrt{x}+\sqrt{y}} \right) = t^{\frac{1}{2}} z(x, y)$$

$\therefore z(x, y)$  is a homogeneous function in of degree  $\frac{1}{2}$ .

∴ By Euler's theorem,  $x \frac{\partial z}{\partial x} + y \frac{\partial z}{\partial y} = \frac{1}{2} z$

$$\text{Put } z = \sin u \Rightarrow x \frac{\partial(\sin u)}{\partial x} + y \frac{\partial(\sin u)}{\partial y} = \frac{1}{2} \sin u$$

$$x \cos u \frac{\partial u}{\partial x} + y \cos u \frac{\partial u}{\partial y} = \frac{1}{2} \sin u$$

$$x \frac{\partial u}{\partial x} + y \frac{\partial u}{\partial y} = \frac{1}{2} \frac{\sin u}{\cos u}$$

$$= \frac{1}{2} \tan u = f(u)$$

By Euler's extension theorem

$$\begin{aligned} x^2 \frac{\partial^2 u}{\partial x^2} + 2xy \frac{\partial^2 u}{\partial x \partial y} + y^2 \frac{\partial^2 u}{\partial y^2} &= f(u)[f'(u) - 1] \\ &= \frac{1}{2} \tan u \left( \frac{1}{2} \sec^2 u - 1 \right) \\ &= \frac{1}{2} \frac{\sin u}{\cos u} \left( \frac{1}{2 \cos^2 u} - 1 \right) \\ &= \frac{1}{2} \frac{\sin u}{\cos u} \left( \frac{1 - 2 \cos^2 u}{2 \cos^2 u} \right) \\ &= \frac{1}{4} \frac{\sin u (-\cos 2u)}{\cos^3 u} \\ &= \frac{-\sin u \cos 2u}{4 \cos^3 u} \end{aligned}$$

Hence proved.

**Example:**

If  $u = (x - y)f\left(\frac{y}{x}\right)$ , then find  $x^2 \frac{\partial^2 u}{\partial x^2} + 2xy \frac{\partial^2 u}{\partial x \partial y} + y^2 \frac{\partial^2 u}{\partial y^2}$  [AU May 2001, Dec 2014]

**Solution:**

$$\text{Given } u(x, y) = (x - y)f\left(\frac{y}{x}\right)$$

$$\begin{aligned} u(tx, ty) &= (tx - ty)f\left(\frac{ty}{tx}\right) \\ &= t^1 u(x, y) \end{aligned}$$

∴  $u(x, y)$  is a homogeneous function in of degree '1'.

∴ By Euler's theorem,  $x \frac{\partial u}{\partial x} + y \frac{\partial u}{\partial y} = 1 \cdot u = u = f(u)$

By Euler's extension theorem

$$\begin{aligned} x^2 \frac{\partial^2 u}{\partial x^2} + 2xy \frac{\partial^2 u}{\partial x \partial y} + y^2 \frac{\partial^2 u}{\partial y^2} &= f(u)[f'(u) - 1] \\ &= u(1 - 1) = u \cdot 0 = 0 \end{aligned}$$